<?xml version="1.0"?>
<rdf:RDF xmlns="hhttps://w3id.org/udo#"
     xml:base="hhttps://w3id.org/udo"
     xmlns:owl="http://www.w3.org/2002/07/owl#"
     xmlns:rdf="http://www.w3.org/1999/02/22-rdf-syntax-ns#"
     xmlns:xml="http://www.w3.org/XML/1998/namespace"
     xmlns:xsd="http://www.w3.org/2001/XMLSchema#"
     xmlns:foaf="http://xmlns.com/foaf/0.1/"
     xmlns:rdfs="http://www.w3.org/2000/01/rdf-schema#"
     xmlns:vann="http://purl.org/vocab/vann/"
     xmlns:terms="http://purl.org/dc/terms/">
    <owl:Ontology rdf:about="hhttps://w3id.org/udo">
        <owl:versionIRI rdf:resource="https://w3id.org/udo/0.2"/>
        <terms:creator rdf:nodeID="genid1"/>
        <terms:description xml:lang="en">Ontology that defines classes for uncertainties in damage assessment</terms:description>
        <terms:license>https://creativecommons.org/licenses/by/1.0</terms:license>
        <terms:title xml:lang="en">Uncertain Damage Ontology</terms:title>
        <vann:preferredNamespacePrefix>udo</vann:preferredNamespacePrefix>
        <vann:preferredNamespaceUri>https://w3id.org/udo#</vann:preferredNamespaceUri>
    </owl:Ontology>
    <rdf:Description rdf:nodeID="genid1">
        <rdf:type rdf:resource="http://xmlns.com/foaf/0.1/Person"/>
        <foaf:name>Al-Hakam Hamdan</foaf:name>
    </rdf:Description>
    


    <!-- 
    ///////////////////////////////////////////////////////////////////////////////////////
    //
    // Annotation properties
    //
    ///////////////////////////////////////////////////////////////////////////////////////
     -->


    


    <!-- http://purl.org/dc/terms/creator -->


    <owl:AnnotationProperty rdf:about="http://purl.org/dc/terms/creator"/>
    


    <!-- http://purl.org/dc/terms/description -->


    <owl:AnnotationProperty rdf:about="http://purl.org/dc/terms/description"/>
    


    <!-- http://purl.org/dc/terms/license -->


    <owl:AnnotationProperty rdf:about="http://purl.org/dc/terms/license"/>
    


    <!-- http://purl.org/dc/terms/title -->


    <owl:AnnotationProperty rdf:about="http://purl.org/dc/terms/title"/>
    


    <!-- http://purl.org/vocab/vann/preferredNamespacePrefix -->


    <owl:AnnotationProperty rdf:about="http://purl.org/vocab/vann/preferredNamespacePrefix"/>
    


    <!-- http://purl.org/vocab/vann/preferredNamespaceUri -->


    <owl:AnnotationProperty rdf:about="http://purl.org/vocab/vann/preferredNamespaceUri"/>
    


    <!-- http://xmlns.com/foaf/0.1/name -->


    <owl:AnnotationProperty rdf:about="http://xmlns.com/foaf/0.1/name"/>
    


    <!-- 
    ///////////////////////////////////////////////////////////////////////////////////////
    //
    // Object Properties
    //
    ///////////////////////////////////////////////////////////////////////////////////////
     -->


    


    <!-- https://w3id.org/udo#hasContradictions -->


    <owl:ObjectProperty rdf:about="https://w3id.org/udo#hasContradictions">
        <rdfs:domain rdf:resource="https://w3id.org/udo#AmbigiousDamage"/>
        <rdfs:range rdf:resource="https://w3id.org/udo#ContradictingDamageClassList"/>
        <rdfs:comment xml:lang="en">References a list of contradicting damage classes that could possibly be determined for an ambigious damage (represented by an instance of udo:AmbigiousDamage).</rdfs:comment>
        <rdfs:label xml:lang="en">has contradictions</rdfs:label>
    </owl:ObjectProperty>
    


    <!-- https://w3id.org/udo#hasUncertainValue -->


    <owl:ObjectProperty rdf:about="https://w3id.org/udo#hasUncertainValue">
        <rdfs:domain rdf:resource="https://w3id.org/udo#UndetectedDamage"/>
        <rdfs:range rdf:resource="https://w3id.org/udo#UncertainValue"/>
        <rdfs:comment xml:lang="en">Assigns a fuzzy value that characterizes an undetected damage (represented through an instance of udo:UndetectedDamage).</rdfs:comment>
        <rdfs:label xml:lang="en">has uncertain value</rdfs:label>
    </owl:ObjectProperty>
    


    <!-- https://w3id.org/udo#hasUndetectedDamage -->


    <owl:ObjectProperty rdf:about="https://w3id.org/udo#hasUndetectedDamage">
        <rdfs:subPropertyOf rdf:resource="https://www.w3id.org/dot#hasDamage"/>
        <rdfs:range rdf:resource="https://w3id.org/udo#UndetectedDamage"/>
        <rdfs:comment xml:lang="en">The relationship between a potentially damaged component and an undetected damage.</rdfs:comment>
        <rdfs:label xml:lang="en">has undetected damage</rdfs:label>
    </owl:ObjectProperty>
    


    <!-- https://w3id.org/udo#referencedDataProperty -->


    <owl:ObjectProperty rdf:about="https://w3id.org/udo#referencedDataProperty">
        <rdfs:domain rdf:resource="https://w3id.org/udo#UncertainValue"/>
        <rdfs:range rdf:resource="http://www.w3.org/2002/07/owl#DatatypeProperty"/>
        <rdfs:comment xml:lang="en">References a specific owl:DataTypeProperty that is used for an uncertain value (represented by an instance of udo:UncertainValue).</rdfs:comment>
        <rdfs:label xml:lang="en">referenced DataProperty</rdfs:label>
    </owl:ObjectProperty>
    


    <!-- https://w3id.org/udo#referencesClass -->


    <owl:ObjectProperty rdf:about="https://w3id.org/udo#referencesClass">
        <rdfs:domain rdf:resource="https://w3id.org/udo#ContradictingDamageClassList"/>
        <rdfs:range rdf:resource="http://www.w3.org/2002/07/owl#Class"/>
        <rdfs:comment xml:lang="en">References an owl:Class that is part of a list of contradicting damage classes for an ambigious damage. The instance of owl:Class should be a subclass of dot:Damage.</rdfs:comment>
        <rdfs:label xml:lang="en">references class</rdfs:label>
    </owl:ObjectProperty>
    


    <!-- https://www.w3id.org/dot#hasDamage -->


    <owl:ObjectProperty rdf:about="https://www.w3id.org/dot#hasDamage"/>
    


    <!-- 
    ///////////////////////////////////////////////////////////////////////////////////////
    //
    // Data properties
    //
    ///////////////////////////////////////////////////////////////////////////////////////
     -->


    


    <!-- https://w3id.org/udo#damagePossibility -->


    <owl:DatatypeProperty rdf:about="https://w3id.org/udo#damagePossibility">
        <rdfs:domain rdf:resource="https://w3id.org/udo#UndetectedDamage"/>
        <rdfs:comment xml:lang="en">The possibility that an Undetected Damage can exist.</rdfs:comment>
        <rdfs:label xml:lang="en">damage possibility</rdfs:label>
    </owl:DatatypeProperty>
    


    <!-- https://w3id.org/udo#damagePossibilityFactor -->


    <owl:DatatypeProperty rdf:about="https://w3id.org/udo#damagePossibilityFactor">
        <rdfs:domain rdf:resource="https://w3id.org/udo#UndetectedDamage"/>
        <rdfs:comment xml:lang="en">An auxiliary parameter that defines a partial possibility of occurence for a damage, usually inferred by a single damage assessment rule. The sum of all possibility factors of an instance of udo:UndetectedDamage can be used in conjunction with an appropriate membership function to determine the overall possibility.</rdfs:comment>
        <rdfs:label xml:lang="en">damage possibility factor</rdfs:label>
    </owl:DatatypeProperty>
    


    <!-- https://w3id.org/udo#damageProbability -->


    <owl:DatatypeProperty rdf:about="https://w3id.org/udo#damageProbability">
        <rdfs:domain rdf:resource="https://w3id.org/udo#UndetectedDamage"/>
        <rdfs:comment xml:lang="en">The probability that an Undetected Damage will exist.</rdfs:comment>
        <rdfs:label xml:lang="en">damage probability</rdfs:label>
    </owl:DatatypeProperty>
    


    <!-- https://w3id.org/udo#enumeration -->


    <owl:DatatypeProperty rdf:about="https://w3id.org/udo#enumeration">
        <rdfs:domain rdf:resource="https://w3id.org/udo#UncertainValue"/>
        <rdfs:comment xml:lang="en">References multiple values that could be set for an uncertain value (represented by an instance of udo:UncertainValue)</rdfs:comment>
        <rdfs:label xml:lang="en">enumeration</rdfs:label>
    </owl:DatatypeProperty>
    


    <!-- https://w3id.org/udo#maxValue -->


    <owl:DatatypeProperty rdf:about="https://w3id.org/udo#maxValue">
        <rdfs:domain rdf:resource="https://w3id.org/udo#UncertainValue"/>
        <rdfs:comment xml:lang="en">Maximum value of a value range that could be set for an uncertain value (represented by an instance of udo:UncertainValue)</rdfs:comment>
        <rdfs:label xml:lang="en">maximum value</rdfs:label>
    </owl:DatatypeProperty>
    


    <!-- https://w3id.org/udo#minValue -->


    <owl:DatatypeProperty rdf:about="https://w3id.org/udo#minValue">
        <rdfs:domain rdf:resource="https://w3id.org/udo#UncertainValue"/>
        <rdfs:comment xml:lang="en">Minimum value of a value range that could be set for an uncertain value (represented by an instance of udo:UncertainValue)</rdfs:comment>
        <rdfs:label xml:lang="en">minimum value</rdfs:label>
    </owl:DatatypeProperty>
    


    <!-- https://w3id.org/udo#overallDamagePossibility -->


    <owl:DatatypeProperty rdf:about="https://w3id.org/udo#overallDamagePossibility">
        <rdfs:domain rdf:resource="https://w3id.org/udo#UndetectedDamage"/>
        <rdfs:comment xml:lang="en">The overall possibility that an Undetected Damage will exist. Sum of all related damage possibilities</rdfs:comment>
        <rdfs:label xml:lang="en">overall damage possibility</rdfs:label>
    </owl:DatatypeProperty>
    


    <!-- https://w3id.org/udo#overallDamageProbability -->


    <owl:DatatypeProperty rdf:about="https://w3id.org/udo#overallDamageProbability">
        <rdfs:domain rdf:resource="https://w3id.org/udo#UndetectedDamage"/>
        <rdfs:comment xml:lang="en">The overall probability that an Undetected Damage will exist. Sum of all related damage probabilities</rdfs:comment>
        <rdfs:label xml:lang="en">overall damage probability</rdfs:label>
    </owl:DatatypeProperty>
    


    <!-- 
    ///////////////////////////////////////////////////////////////////////////////////////
    //
    // Classes
    //
    ///////////////////////////////////////////////////////////////////////////////////////
     -->


    


    <!-- http://www.w3.org/2002/07/owl#Class -->


    <owl:Class rdf:about="http://www.w3.org/2002/07/owl#Class"/>
    


    <!-- http://www.w3.org/2002/07/owl#DatatypeProperty -->


    <owl:Class rdf:about="http://www.w3.org/2002/07/owl#DatatypeProperty"/>
    


    <!-- http://xmlns.com/foaf/0.1/Person -->


    <owl:Class rdf:about="http://xmlns.com/foaf/0.1/Person"/>
    


    <!-- https://w3id.org/udo#AmbigiousDamage -->


    <owl:Class rdf:about="https://w3id.org/udo#AmbigiousDamage">
        <rdfs:subClassOf rdf:resource="https://www.w3id.org/dot#Damage"/>
        <rdfs:comment xml:lang="en">A Damage that is not further classified with domain-specific classes</rdfs:comment>
        <rdfs:label xml:lang="en">Ambigious Damage</rdfs:label>
    </owl:Class>
    


    <!-- https://w3id.org/udo#ContradictingDamageClassList -->


    <owl:Class rdf:about="https://w3id.org/udo#ContradictingDamageClassList">
        <rdfs:comment xml:lang="en">Functions as List that references contradicting damage classes (subclasses of dot:Damage) for a specific instance of udo:AmbigiousDamage</rdfs:comment>
        <rdfs:label xml:lang="en">Contradicting Damage Class List</rdfs:label>
    </owl:Class>
    


    <!-- https://w3id.org/udo#UncertainValue -->


    <owl:Class rdf:about="https://w3id.org/udo#UncertainValue">
        <rdfs:comment xml:lang="en">An auxiliary class for instantiating value objects that contain fuzzyness, e.g. a fuzzy value or reference. Thus an instance of udo:UncertainValue can reference value ranges (min and max) or enumerations.</rdfs:comment>
        <rdfs:label xml:lang="en">Uncertain Value</rdfs:label>
    </owl:Class>
    


    <!-- https://w3id.org/udo#UndetectedDamage -->


    <owl:Class rdf:about="https://w3id.org/udo#UndetectedDamage">
        <rdfs:subClassOf rdf:resource="https://www.w3id.org/dot#Damage"/>
        <rdfs:comment xml:lang="en">A Damage that has not been asserted or detected through inspections and therefore can only be reasoned by other facts.</rdfs:comment>
        <rdfs:label xml:lang="en">Undetected Damage</rdfs:label>
    </owl:Class>
    


    <!-- https://w3id.org/udo#UnidentifiedDamage -->


    <owl:Class rdf:about="https://w3id.org/udo#UnidentifiedDamage">
        <rdfs:subClassOf rdf:resource="https://www.w3id.org/dot#Damage"/>
        <rdfs:comment xml:lang="en">A Damage which has multiple asserted domain-specific classes, so that an unambigious classification of the respective Damage instance is not possible.</rdfs:comment>
        <rdfs:label xml:lang="en">Unidentified Damage</rdfs:label>
    </owl:Class>
    


    <!-- https://www.w3id.org/dot#Damage -->


    <owl:Class rdf:about="https://www.w3id.org/dot#Damage"/>
</rdf:RDF>



<!-- Generated by the OWL API (version 5.1.18) https://github.com/owlcs/owlapi/ -->


